DynamoDbEncryption/runtimes/java/src/main/smithy-generated/software/amazon/cryptography/dynamoDbEncryption/model/LegacyPolicy.java
@@ -1,7 +1,7 @@
 // Copyright Amazon.com Inc. or its affiliates. All Rights Reserved.
 // SPDX-License-Identifier: Apache-2.0
 // Do not modify this file. This file is machine generated, and any changes to it will be overwritten.
-package software.amazon.cryptography.dynamoDbEncryption.itemEncryptor.model;
+package software.amazon.cryptography.dynamoDbEncryption.model;
 
 public enum LegacyPolicy {
   REQUIRE_ENCRYPT_ALLOW_DECRYPT("REQUIRE_ENCRYPT_ALLOW_DECRYPT"),
