DynamoDbEncryption/Model/AwsCryptographyDynamoDbEncryptionItemEncryptorTypes.dfy
@@ -102,7 +102,7 @@ include "../../submodules/MaterialProviders/StandardLibrary/src/Index.dfy"
  nameonly algorithmSuiteId: Option<AwsCryptographyMaterialProvidersTypes.DBEAlgorithmSuiteId> ,
  nameonly keyring: Option<AwsCryptographyMaterialProvidersTypes.IKeyring> ,
  nameonly cmm: Option<AwsCryptographyMaterialProvidersTypes.ICryptographicMaterialsManager> ,
- nameonly legacyConfig: Option<LegacyConfig>
+ nameonly legacyConfig: Option<AwsCryptographyDynamoDbEncryptionTypes.LegacyConfig>
  )
  datatype EncryptItemInput = | EncryptItemInput (
  nameonly plaintextItem: ComAmazonawsDynamodbTypes.AttributeMap
@@ -110,51 +110,6 @@ include "../../submodules/MaterialProviders/StandardLibrary/src/Index.dfy"
  datatype EncryptItemOutput = | EncryptItemOutput (
  nameonly encryptedItem: ComAmazonawsDynamodbTypes.AttributeMap
  )
- datatype LegacyConfig = | LegacyConfig (
- nameonly policy: LegacyPolicy ,
- nameonly encryptor: ILegacyDynamoDbEncryptor ,
- nameonly attributeFlags: AwsCryptographyDynamoDbEncryptionTypes.AttributeActions ,
- nameonly defaultAttributeFlag: Option<AwsCryptographyStructuredEncryptionTypes.CryptoAction>
- )
- class ILegacyDynamoDbEncryptorCallHistory {
- ghost constructor() {
- 
-}
- 
-}
- trait {:termination false} ILegacyDynamoDbEncryptor
- {
- // Helper to define any additional modifies/reads clauses.
- // If your operations need to mutate state,
- // add it in your constructor function:
- // Modifies := {your, fields, here, History};
- // If you do not need to mutate anything:
-// Modifies := {History};
-
- ghost const Modifies: set<object>
- // For an unassigned field defined in a trait,
- // Dafny can only assign a value in the constructor.
- // This means that for Dafny to reason about this value,
- // it needs some way to know (an invariant),
- // about the state of the object.
- // This builds on the Valid/Repr paradigm
- // To make this kind requires safe to add
- // to methods called from unverified code,
- // the predicate MUST NOT take any arguments.
- // This means that the correctness of this requires
- // MUST only be evaluated by the class itself.
- // If you require any additional mutation,
- // then you MUST ensure everything you need in ValidState.
- // You MUST also ensure ValidState in your constructor.
- predicate ValidState()
- ensures ValidState() ==> History in Modifies
-  ghost const History: ILegacyDynamoDbEncryptorCallHistory
- 
-}
- datatype LegacyPolicy =
-	| REQUIRE_ENCRYPT_ALLOW_DECRYPT
-	| FORBID_ENCRYPT_ALLOW_DECRYPT
-	| FORBID_ENCRYPT_FORBID_DECRYPT
  datatype Error =
  // Local Error structures are listed here
  | DynamoDbItemEncryptorException (
