DynamoDbEncryption/Model/AwsCryptographyDynamoDbEncryptionTypes.dfy
@@ -141,6 +141,51 @@ include "../../submodules/MaterialProviders/StandardLibrary/src/Index.dfy"
  datatype Insert = | Insert (
  nameonly literal: string
  )
+ datatype LegacyConfig = | LegacyConfig (
+ nameonly policy: LegacyPolicy ,
+ nameonly encryptor: ILegacyDynamoDbEncryptor ,
+ nameonly attributeFlags: AttributeActions ,
+ nameonly defaultAttributeFlag: Option<AwsCryptographyStructuredEncryptionTypes.CryptoAction>
+ )
+ class ILegacyDynamoDbEncryptorCallHistory {
+ ghost constructor() {
+ 
+}
+ 
+}
+ trait {:termination false} ILegacyDynamoDbEncryptor
+ {
+ // Helper to define any additional modifies/reads clauses.
+ // If your operations need to mutate state,
+ // add it in your constructor function:
+ // Modifies := {your, fields, here, History};
+ // If you do not need to mutate anything:
+// Modifies := {History};
+
+ ghost const Modifies: set<object>
+ // For an unassigned field defined in a trait,
+ // Dafny can only assign a value in the constructor.
+ // This means that for Dafny to reason about this value,
+ // it needs some way to know (an invariant),
+ // about the state of the object.
+ // This builds on the Valid/Repr paradigm
+ // To make this kind requires safe to add
+ // to methods called from unverified code,
+ // the predicate MUST NOT take any arguments.
+ // This means that the correctness of this requires
+ // MUST only be evaluated by the class itself.
+ // If you require any additional mutation,
+ // then you MUST ensure everything you need in ValidState.
+ // You MUST also ensure ValidState in your constructor.
+ predicate ValidState()
+ ensures ValidState() ==> History in Modifies
+  ghost const History: ILegacyDynamoDbEncryptorCallHistory
+ 
+}
+ datatype LegacyPolicy =
+	| REQUIRE_ENCRYPT_ALLOW_DECRYPT
+	| FORBID_ENCRYPT_ALLOW_DECRYPT
+	| FORBID_ENCRYPT_FORBID_DECRYPT
  datatype Lower = | Lower (
  
  )
