DynamoDbEncryption/src/DynamoDbItemEncryptor/InternalLegacyConfig.dfy
@@ -1,18 +1,19 @@
 // Copyright Amazon.com Inc. or its affiliates. All Rights Reserved.
 // SPDX-License-Identifier: Apache-2.0
 
-include "../Model/AwsCryptographyDynamoDbItemEncryptorTypes.dfy"
+include "../../Model/AwsCryptographyDynamoDbEncryptionItemEncryptorTypes.dfy"
 
-module {:extern "Dafny.Aws.Cryptography.DynamoDbItemEncryptor.Internal"} InternalLegacyConfig {
+module {:extern "Dafny.Aws.Cryptography.DynamoDbEncryption.ItemEncryptor.Internal"} InternalLegacyConfig {
   import opened Wrappers
-  import Types = AwsCryptographyDynamoDbItemEncryptorTypes
+  import Types = AwsCryptographyDynamoDbEncryptionItemEncryptorTypes
+  import DDBE = AwsCryptographyDynamoDbEncryptionTypes
 
   class {:extern} InternalLegacyConfig {
 
     static method {:extern} Build(encryptorConfig: Types.DynamoDbItemEncryptorConfig)
       returns (output: Result<Option<InternalLegacyConfig>, Types.Error>)
 
-    const policy: Types.LegacyPolicy
+    const policy: DDBE.LegacyPolicy
 
     method {:extern} EncryptItem(input: Types.EncryptItemInput)
       returns (output: Result<Types.EncryptItemOutput, Types.Error>)
