DynamoDbEncryption/test/TestFixtures.dfy
@@ -34,7 +34,8 @@ module TestFixtures {
       allowedUnauthenticatedAttributePrefix := None(),
       keyring := Some(keyring),
       cmm := None(),
-      algorithmSuiteId := None()
+      algorithmSuiteId := None(),
+      legacyConfig := None()
     );
   }
 
@@ -54,7 +55,8 @@ module TestFixtures {
       allowedUnauthenticatedAttributePrefix := config.allowedUnauthenticatedAttributePrefix,
       keyring := Some(keyring),
       cmm := None(),
-      algorithmSuiteId := None()
+      algorithmSuiteId := None(),
+      legacyConfig := None()
     );
     encryptor :- expect DynamoDbItemEncryptor.DynamoDbItemEncryptor(encryptorConfig);
   }
@@ -163,46 +165,6 @@ module TestFixtures {
           )
         ]
       )
-  }
-  
-  function method GetAttributeActions() : Types.AttributeActions {
-    map["bar" := CTypes.SIGN_ONLY, "encrypt" := CTypes.ENCRYPT_AND_SIGN, "sign" := CTypes.SIGN_ONLY, "nothing" := CTypes.DO_NOTHING]
-  }
-
-  method GetEncryptorConfig() returns (output : Types.DynamoDbItemEncryptorConfig) {
-    var keyring := GetKmsKeyring();
-    output := Types.DynamoDbItemEncryptorConfig(
-      tableName := "foo",
-      partitionKeyName := "bar",
-      sortKeyName := None(),
-      attributeActions := GetAttributeActions(),
-      allowedUnauthenticatedAttributes := Some(["nothing"]),
-      allowedUnauthenticatedAttributePrefix := None(),
-      keyring := Some(keyring),
-      cmm := None(),
-      algorithmSuiteId := None(),
-      legacyConfig := None()
-    );
-  }
-
-  method GetDynamoDbItemEncryptorFrom(config : Types.DynamoDbItemEncryptorConfig)
-    returns (encryptor: DynamoDbItemEncryptor.DynamoDbItemEncryptorClient)
-    ensures encryptor.ValidState()
-    ensures fresh(encryptor)
-    ensures fresh(encryptor.Modifies)
-  {
-    var keyring := GetKmsKeyring();
-    var encryptorConfig := Types.DynamoDbItemEncryptorConfig(
-      tableName := config.tableName,
-      partitionKeyName := config.partitionKeyName,
-      sortKeyName := config.sortKeyName,
-      attributeActions := config.attributeActions,
-      allowedUnauthenticatedAttributes := config.allowedUnauthenticatedAttributes,
-      allowedUnauthenticatedAttributePrefix := config.allowedUnauthenticatedAttributePrefix,
-      keyring := Some(keyring),
-      cmm := None(),
-      algorithmSuiteId := None(),
-      legacyConfig := None()
     );
   }
 }
