DynamoDbEncryption/Model/DynamoDbEncryption.smithy
@@ -72,6 +72,40 @@ map AttributeActions {
     value: CryptoAction,
 }
 
+@enum([
+  {
+    name: "REQUIRE_ENCRYPT_ALLOW_DECRYPT",
+    value: "REQUIRE_ENCRYPT_ALLOW_DECRYPT",
+  },
+  {
+    name: "FORBID_ENCRYPT_ALLOW_DECRYPT",
+    value: "FORBID_ENCRYPT_ALLOW_DECRYPT",
+  },
+  {
+    name: "FORBID_ENCRYPT_FORBID_DECRYPT",
+    value: "FORBID_ENCRYPT_FORBID_DECRYPT",
+  },
+])
+string LegacyPolicy
+
+@aws.polymorph#extendable
+resource LegacyDynamoDbEncryptor {
+    operations: []
+}
+
+@aws.polymorph#reference(resource: LegacyDynamoDbEncryptor)
+structure LegacyDynamoDbEncryptorReference {}
+
+structure LegacyConfig {
+    @required
+    policy: LegacyPolicy,
+    @required
+    encryptor: LegacyDynamoDbEncryptorReference,
+    @required
+    attributeFlags: AttributeActions,
+    defaultAttributeFlag: CryptoAction,
+}
+
 @range(min: 1, max: 63)
 integer BeaconBitLength
 
